- Subtyping check failed - Expected type     predicate:     refined_child_node_predicate t       (fun parent1 child1 ->           is_equal_node csn parent1 && is_child parent1 child1) {_ << lv}   got type     refined_child_node_predicate t       (fun parent1 child1 ->           is_equal_node parent parent1 && is_child parent1 child1)

src/study/Nemonuri.Study.CSharpSyntaxRewriter2.Modifier/Nemonuri.StratifiedNode.IndexTheory.Base.fst
@@ -8,6 +8,10 @@ open Nemonuri.StratifiedNode.NodeTheory
 
 let stratified_node_indexes = list nat
 
+let add_index (sni:stratified_node_indexes) (index:nat) = L.append sni [index]
+
+let empty_stratified_node_indexes : stratified_node_indexes = []
+
 let convert_level_to_indexes_length (level:pos)
   : Tot nat
   = level - 1
@@ -60,11 +64,11 @@ let rec get_node_from_indexes
       let next_sn = get_child_at sn child_index in
       get_node_from_indexes next_sn next_sni
 
-private let rec try_get_index_in_children_core
+private let rec try_get_index_of_child_from_predicate_core
   (#t:eqtype) (#lv:pos) (parent:stratified_node t lv) 
   (#children_mlv:nat)
   (subchildren:stratified_node_list t children_mlv{ is_subchildren parent subchildren })
-  (predicate:(child_node_predicate parent))
+  (predicate:refined_child_node_predicate t (fun parent1 child1 -> (is_equal_node parent parent1) && (is_child parent1 child1)))
   : Tot (option (child_node_index parent)) 
         (decreases subchildren)
   = if is_empty subchildren then 
@@ -72,26 +76,66 @@ private let rec try_get_index_in_children_core
     else
       (
         lemma_for_subchildren parent subchildren;
-        if predicate (get_hd subchildren) then 
+        if predicate parent (get_hd subchildren) then 
           Some ((get_children_length parent) - (get_length subchildren))
         else 
-          try_get_index_in_children_core parent (get_tl subchildren) predicate
+          try_get_index_of_child_from_predicate_core parent (get_tl subchildren) predicate
       )
 
-let try_get_index_in_children
+let try_get_index_of_child_from_predicate
   (#t:eqtype) (#lv:pos) (parent:stratified_node t lv)
-  (predicate:(child_node_predicate parent))
+  (predicate:refined_child_node_predicate t (fun parent1 child1 -> (is_equal_node parent parent1) && (is_child parent1 child1)))
   : Tot (option (child_node_index parent)) 
-  = try_get_index_in_children_core parent parent.children predicate
+  = try_get_index_of_child_from_predicate_core parent parent.children predicate
 
+#push-options "--query_stats"
+let rec try_get_indexes_of_descendant_or_self_from_predicate_core
+  (#t:eqtype) (#lv:pos) (parent:stratified_node t lv) (parent_indexes:stratified_node_indexes)
+  (predicate:refined_child_node_predicate t (fun parent1 child1 -> (is_equal_node parent parent1) && (is_child parent1 child1)))
+  : Tot (option (stratified_node_indexes)) 
+        (decreases lv)
+  = match (try_get_index_of_child_from_predicate parent predicate) with
+  | Some v1 -> Some (add_index parent_indexes v1)
+  | None -> 
+    let v2 =
+      select_in_children parent (
+        fun psn csn -> (
+          lemma_child_node_level_is_lower_than_parent psn csn;
+          assert (lv > (get_level csn));
+          let cni = get_child_node_index csn in
+          let new_parent_indexes = add_index parent_indexes cni in
+          try_get_indexes_of_descendant_or_self_from_predicate_core csn new_parent_indexes predicate
+        )
+      ) in
+    let v3 = L.find (Some?) v2 in
+    match v3 with
+    | None -> None
+    | Some v4 -> v4
+#pop-options
+      
+      
+//let cnp = convert_stratified_node_predicate_to_child_node_predicate predicate sn in
 
 (*
-let rec try_get_indexes_from_predicate
-  (#t:eqtype) (#lv:pos) (sn:stratified_node t lv)
+let rec try_get_indexes_of_descendant_or_self_from_predicate
+  (#t:eqtype) (#lv:pos) (root:stratified_node t lv)
   (predicate:stratified_node_predicate t)
-  : Tot (option (sni:stratified_node_indexes{ contains_indexes sn sni }))
-  = 
+  : Tot (option (stratified_node_indexes)) 
+  = if (predicate root) then
+      Some empty_stratified_node_indexes
+    else
 *)
+
+(*
+  = match (if (predicate parent) then (Some empty_stratified_node_indexes) else None) with
+  | None -> None
+  | Some v1 ->
+      let cnp = convert_stratified_node_predicate_to_child_node_predicate predicate parent in
+      match (try_get_index_of_child_from_predicate parent cnp) with
+      | None -> None
+      | Some v2 -> 
+*)    
+
 
 (*
 let rec get_indexes_from_node
