src/study/Nemonuri.Study.CSharpSyntaxRewriter2.Modifier/Nemonuri.StratifiedNode.NodeTheory.Child.fst
@@ -5,33 +5,122 @@ open Nemonuri.StratifiedNode
 open Nemonuri.StratifiedNode.ListTheory
 open Nemonuri.StratifiedNode.NodeTheory.Common
 
-let child_level (parent_level:pos) = cl:pos{ cl < parent_level }
+let is_child_level (parent_level:pos) (cl:pos) : Tot bool = cl < parent_level 
+
+(*
+let child_level (parent_level:pos) = cl:pos{ is_child_level parent_level cl}
+*)
 
 let child_node
-  (#t:eqtype) (#parent_level:pos) 
-  (parent:stratified_node t parent_level)
-  (clv:(child_level parent_level)) =
-    (cn:(stratified_node t clv){ is_child parent cn })
+  (#t:eqtype) 
+  (#parent_level:pos) (parent:stratified_node t parent_level)
+  (child_level:pos) =
+  (cn:(stratified_node t child_level){ is_child parent cn })
+
+let is_child_node_index 
+  (#t:eqtype) (#parent_level:pos) (parent:stratified_node t parent_level)
+  (cni:nat)
+  : Tot bool
+  = cni < (get_children_length parent)
 
 let child_node_index 
   (#t:eqtype) (#parent_level:pos) (parent:stratified_node t parent_level) =
-  nat1:nat{ nat1 < (get_children_length parent) }
+  nat1:nat{ is_child_node_index parent nat1 }
+
+let get_child_node_index
+  (#t:eqtype) (#parent_level:pos) 
+  (#parent:stratified_node t parent_level)
+  (#child_level:pos)
+  (cn:child_node parent child_level)
+  : Tot (child_node_index parent)
+  = index_of parent.children cn
 
 let child_node_func
-  (#t:eqtype) (#parent_level:pos) (parent:stratified_node t parent_level) (t2:Type) =
-    (#clv:(child_level parent_level)) ->
-    (cn:(child_node parent clv)) ->
+  (t:eqtype) (t2:Type) =
+    (#parent_level:pos) ->
+    (parent:stratified_node t parent_level) ->
+    (#child_level:pos) ->
+    (cn:(child_node parent child_level)) ->
     Tot t2
 
-let child_node_predicate
-  (#t:eqtype) (#parent_level:pos) (parent:stratified_node t parent_level) =
-  child_node_func parent bool
+(*
+let parent_bound_child_node_func
+  (t:eqtype) (t2:Type)
+  (#parent_level:pos) (parent:stratified_node t parent_level)
+  = (refined_stratified_node_func t t2 (is_child parent))
+
+let bound_parent
+  (#t:eqtype) (#t2:Type) (#parent_level:pos) (parent:stratified_node t parent_level)
+  (cnf:child_node_func t t2)
+  : Tot (parent_bound_child_node_func t t2 parent)
+  = cnf parent
+
+noeq
+type parent_bound_child_node_func_info (t:eqtype) (t2:Type) (#parent_level:pos) (parent:stratified_node t parent_level) 
+= {
+  original_func: (child_node_func t t2);
+  bound_func: (parent_bound_child_node_func t t2 parent)
+}
+*)
+
+(*
+let to_stratified_node_func
+  (#t:eqtype) (#t2:Type) (cnf:child_node_func t t2)
+  (#parent_level:pos) (parent:stratified_node t parent_level)
+  : Tot (stratified_node_func t t2)
+  = cnf #parent_level parent
+*)
+
+(*
+let child_node_and_index_func
+  (t:eqtype) (t2:Type) =
+    (#parent_level:pos) ->
+    (parent:stratified_node t parent_level) ->
+    (#clv:(child_level parent_level)) ->
+    (cn:(child_node parent clv)) ->
+    (cni:(child_node_index parent){get_child_node_index cn = cni}) ->
+    Tot t2
+*)
+
+let child_node_predicate (t:eqtype) =
+  child_node_func t bool
+
+let refined_child_node_func
+  (t:eqtype) (t2:Type) (predicate:child_node_predicate t) =
+  (#parent_level:pos) ->
+  (parent:stratified_node t parent_level) ->
+  (#child_level:pos) ->
+  (child:(child_node parent child_level){ predicate parent child }) ->
+  Tot t2
+
+let refined_child_node_predicate (t:eqtype) (predicate:child_node_predicate t) =
+  refined_child_node_func t bool predicate
+
+(*
+let convert_stratified_node_predicate_to_child_node_predicate
+  (#t:eqtype) (snp:stratified_node_predicate t)
+  : Tot (child_node_predicate t)
+  = fun 
+      (#parent_level:pos) (parent:stratified_node t parent_level)
+      (#clv:(child_level parent_level)) (cn:(child_node parent clv)) ->
+    (snp #clv cn)
+*)
+
+(*
+type parent_bound_child_node_func (t:eqtype) (t2:Type) =
+  | PBound : 
+    (#parent_level:pos) ->
+    (parent:stratified_node t parent_level) ->
+    (original_func:child_node_func t t2) ->
+    (bound_func:)
+*)
 
 private let rec select_in_children_core
   (#t:eqtype) (#lv:pos) (parent:stratified_node t lv) 
   (#children_mlv:nat)
   (subchildren:stratified_node_list t children_mlv{ is_subchildren parent subchildren })
-  (#t2:Type) (selector:(child_node_func parent t2))
+  (#t2:Type) 
+  (selector:refined_child_node_func t t2 (fun parent1 child1 -> (is_equal_node parent parent1) && (is_child parent1 child1)))
   : Tot (x:(list t2){ L.length x = get_length subchildren }) 
         (decreases subchildren)
   = if is_empty subchildren then 
@@ -40,13 +129,13 @@ private let rec select_in_children_core
       (
         lemma_for_subchildren parent subchildren;
         let hd = get_hd subchildren in
-        (selector #(get_level hd) hd)::
+        (selector parent hd)::
         (select_in_children_core parent (get_tl subchildren) selector)
       )
 
 let select_in_children
-  (#t:eqtype) (#lv:pos) (parent:stratified_node t lv) 
-  (#t2:Type) (selector:(child_node_func parent t2))
+  (#t:eqtype) (#lv:pos) (parent:stratified_node t lv) (#t2:Type)
+  (selector:refined_child_node_func t t2 (fun parent1 child1 -> (is_equal_node parent parent1) && (is_child parent1 child1)))
   : Tot (x:(list t2){ L.length x = get_length parent.children })
   = select_in_children_core parent parent.children selector
 
@@ -54,14 +143,14 @@ private let rec exists_in_children_core
   (#t:eqtype) (#lv:pos) (parent:stratified_node t lv) 
   (#children_mlv:nat)
   (subchildren:stratified_node_list t children_mlv{ is_subchildren parent subchildren })
-  (predicate:(child_node_predicate parent))
+  (predicate:refined_child_node_predicate t (fun parent1 child1 -> (is_equal_node parent parent1) && (is_child parent1 child1)))
   : Tot bool (decreases subchildren)
   = if is_empty subchildren then 
       false
     else
       (
         lemma_for_subchildren parent subchildren;
-        if predicate (get_hd subchildren) then 
+        if predicate parent (get_hd subchildren) then 
           true
         else 
           exists_in_children_core parent (get_tl subchildren) predicate
@@ -69,6 +158,31 @@ private let rec exists_in_children_core
 
 let exists_in_children
   (#t:eqtype) (#lv:pos) (parent:stratified_node t lv)
-  (predicate:(child_node_predicate parent))
+  (predicate:refined_child_node_predicate t (fun parent1 child1 -> (is_equal_node parent parent1) && (is_child parent1 child1)))
   : Tot bool
   = exists_in_children_core parent parent.children predicate
+
+(*
+private let rec select_with_index_in_children_core
+  (#t:eqtype) (#lv:pos) (parent:stratified_node t lv) 
+  (#children_mlv:nat)
+  (subchildren:stratified_node_list t children_mlv{ is_subchildren parent subchildren })
+  (#t2:Type) (selector:(child_node_and_index_func t t2))
+  : Tot (x:(list t2){ L.length x = get_length subchildren }) 
+        (decreases subchildren)
+  = if is_empty subchildren then 
+      []
+    else
+      (
+        lemma_for_subchildren parent subchildren;
+        let hd = get_hd subchildren in
+        (selector parent hd (get_child_node_index hd))::
+        (select_with_index_in_children_core parent (get_tl subchildren) selector)
+      )
+
+let select_with_index_in_children
+  (#t:eqtype) (#lv:pos) (parent:stratified_node t lv) 
+  (#t2:Type) (selector:(child_node_and_index_func t t2))
+  : Tot (x:(list t2){ L.length x = get_length parent.children })
+  = select_with_index_in_children_core parent parent.children selector
+*)
